theories/program_logic/ectx_lifting.v
@@ -1,30 +1,34 @@
 (** Some derived lemmas for ectx-based languages *)
 From iris.proofmode Require Import tactics.
+From iris.program_logic Require Export ectx_language.
 From aneris.program_logic Require Export ectx_language weakestpre lifting.
+Set Default Proof Using "Type".
 
 Section wp.
-Context {Λ : ectxLanguage} `{!irisG Λ Σ} {Hinh : Inhabited (state Λ)}.
+Context {Λ : ectxLanguage} `{!irisG Λ AS Σ} {Hinh : Inhabited (state Λ)}.
 Implicit Types s : stuckness.
 Implicit Types P : iProp Σ.
 Implicit Types Φ : val Λ → iProp Σ.
 Implicit Types v : val Λ.
 Implicit Types e : expr Λ.
 Hint Resolve head_prim_reducible head_reducible_prim_step : core.
-Local Definition reducible_not_val_inhabitant e := reducible_not_val e inhabitant.
+Local Definition reducible_not_val_inhabitant e :=
+  reducible_not_val e inhabitant.
 Hint Resolve reducible_not_val_inhabitant : core.
 Hint Resolve head_stuck_stuck : core.
 
 Lemma wp_lift_head_step_fupd {s E Φ} e1 :
   to_val e1 = None →
-  (∀ σ1 κ κs n, state_interp σ1 (κ ++ κs) n ={E,∅}=∗
+  (∀ σ1 δ1 κ κs n, state_interp σ1 δ1 κs n ={E,∅}=∗
     ⌜head_reducible e1 σ1⌝ ∗
     ∀ e2 σ2 efs, ⌜head_step e1 σ1 κ e2 σ2 efs⌝ ={∅}=∗ ▷ |={∅,E}=>
-      state_interp σ2 κs (length efs + n) ∗
+      ∃ δ2, ⌜valid_state_evolution AS σ1 δ1 κ σ2 δ2⌝ ∗
+      state_interp σ2 δ2 (κs ++ κ) (length efs + n) ∗
       WP e2 @ s; E {{ Φ }} ∗
       [∗ list] ef ∈ efs, WP ef @ s; ⊤ {{ fork_post }})
   ⊢ WP e1 @ s; E {{ Φ }}.
 Proof.
-  iIntros (?) "H". iApply wp_lift_step_fupd=>//. iIntros (σ1 κ κs Qs) "Hσ".
+  iIntros (?) "H". iApply wp_lift_step_fupd=>//. iIntros (σ1 κ κs Qs st) "Hσ".
   iMod ("H" with "Hσ") as "[% H]"; iModIntro.
   iSplit; first by destruct s; eauto. iIntros (e2 σ2 efs ?).
   iApply "H"; eauto.
@@ -32,26 +36,28 @@ Qed.
 
 Lemma wp_lift_head_step {s E Φ} e1 :
   to_val e1 = None →
-  (∀ σ1 κ κs n, state_interp σ1 (κ ++ κs) n ={E,∅}=∗
+  (∀ σ1 δ1 κ κs n, state_interp σ1 δ1 κs n ={E,∅}=∗
     ⌜head_reducible e1 σ1⌝ ∗
     ▷ ∀ e2 σ2 efs, ⌜head_step e1 σ1 κ e2 σ2 efs⌝ ={∅,E}=∗
-      state_interp σ2 κs (length efs + n) ∗
+      ∃ δ2, ⌜valid_state_evolution AS σ1 δ1 κ σ2 δ2⌝ ∗
+      state_interp σ2 δ2 (κs ++ κ) (length efs + n) ∗
       WP e2 @ s; E {{ Φ }} ∗
       [∗ list] ef ∈ efs, WP ef @ s; ⊤ {{ fork_post }})
   ⊢ WP e1 @ s; E {{ Φ }}.
 Proof.
-  iIntros (?) "H". iApply wp_lift_head_step_fupd; [done|]. iIntros (????) "?".
-  iMod ("H" with "[$]") as "[$ H]". iIntros "!>" (e2 σ2 efs ?) "!> !>". by iApply "H".
+  iIntros (?) "H". iApply wp_lift_head_step_fupd; [done|]. iIntros (?????) "?".
+  iMod ("H" with "[$]") as "[$ H]". iIntros "!>" (e2 σ2 efs ?) "!> !>".
+  iApply "H"; done.
 Qed.
 
 Lemma wp_lift_head_stuck E Φ e :
   to_val e = None →
   sub_redexes_are_values e →
-  (∀ σ κs n, state_interp σ κs n ={E,∅}=∗ ⌜head_stuck e σ⌝)
+  (∀ σ κs n st, state_interp σ κs n st ={E,∅}=∗ ⌜head_stuck e σ⌝)
   ⊢ WP e @ E ?{{ Φ }}.
 Proof.
   iIntros (??) "H". iApply wp_lift_stuck; first done.
-  iIntros (σ κs n) "Hσ". iMod ("H" with "Hσ") as "%". by auto.
+  iIntros (σ κs n st) "Hσ". iMod ("H" with "Hσ") as "%". by auto.
 Qed.
 
 Lemma wp_lift_pure_head_stuck E Φ e :
@@ -61,69 +67,81 @@ Lemma wp_lift_pure_head_stuck E Φ e :
   ⊢ WP e @ E ?{{ Φ }}.
 Proof using Hinh.
   iIntros (?? Hstuck). iApply wp_lift_head_stuck; [done|done|].
-  iIntros (σ κs n) "_". iMod (fupd_intro_mask' E ∅) as "_"; first set_solver.
-  by auto.
+  iIntros (σ κs n st) "_". iMod (fupd_intro_mask' E ∅) as "_"; first set_solver.
+  auto; done.
 Qed.
 
 Lemma wp_lift_atomic_head_step_fupd {s E1 E2 Φ} e1 :
   to_val e1 = None →
-  (∀ σ1 κ κs n, state_interp σ1 (κ ++ κs) n ={E1}=∗
+  (∀ σ1 δ1 κ κs n, state_interp σ1 δ1 κs n ={E1}=∗
     ⌜head_reducible e1 σ1⌝ ∗
     ∀ e2 σ2 efs, ⌜head_step e1 σ1 κ e2 σ2 efs⌝ ={E1}[E2]▷=∗
-      state_interp σ2 κs (length efs + n) ∗
+      ∃ δ2, ⌜valid_state_evolution AS σ1 δ1 κ σ2 δ2⌝ ∗
+      state_interp σ2 δ2 (κs ++ κ) (length efs + n) ∗
       from_option Φ False (to_val e2) ∗
       [∗ list] ef ∈ efs, WP ef @ s; ⊤ {{ fork_post }})
   ⊢ WP e1 @ s; E1 {{ Φ }}.
 Proof.
   iIntros (?) "H". iApply wp_lift_atomic_step_fupd; [done|].
-  iIntros (σ1 κ κs Qs) "Hσ1". iMod ("H" with "Hσ1") as "[% H]"; iModIntro.
+  iIntros (σ1 κ κs Qs st) "Hσ1". iMod ("H" with "Hσ1") as "[% H]"; iModIntro.
   iSplit; first by destruct s; auto. iIntros (e2 σ2 efs Hstep).
   iApply "H"; eauto.
 Qed.
 
 Lemma wp_lift_atomic_head_step {s E Φ} e1 :
   to_val e1 = None →
-  (∀ σ1 κ κs n, state_interp σ1 (κ ++ κs) n ={E}=∗
+  (∀ σ1 δ1 κ κs n, state_interp σ1 δ1 κs n ={E}=∗
     ⌜head_reducible e1 σ1⌝ ∗
     ▷ ∀ e2 σ2 efs, ⌜head_step e1 σ1 κ e2 σ2 efs⌝ ={E}=∗
-      state_interp σ2 κs (length efs + n) ∗
+      ∃ δ2, ⌜valid_state_evolution AS σ1 δ1 κ σ2 δ2⌝ ∗
+      state_interp σ2 δ2 (κs ++ κ) (length efs + n) ∗
       from_option Φ False (to_val e2) ∗
       [∗ list] ef ∈ efs, WP ef @ s; ⊤ {{ fork_post }})
   ⊢ WP e1 @ s; E {{ Φ }}.
 Proof.
   iIntros (?) "H". iApply wp_lift_atomic_step; eauto.
-  iIntros (σ1 κ κs Qs) "Hσ1". iMod ("H" with "Hσ1") as "[% H]"; iModIntro.
+  iIntros (σ1 κ κs Qs st) "Hσ1". iMod ("H" with "Hσ1") as "[% H]"; iModIntro.
   iSplit; first by destruct s; auto. iNext. iIntros (e2 σ2 efs Hstep).
   iApply "H"; eauto.
 Qed.
 
 Lemma wp_lift_atomic_head_step_no_fork_fupd {s E1 E2 Φ} e1 :
   to_val e1 = None →
-  (∀ σ1 κ κs n, state_interp σ1 (κ ++ κs) n ={E1}=∗
+  (∀ σ1 δ1 κ κs n, state_interp σ1 δ1 κs n ={E1}=∗
     ⌜head_reducible e1 σ1⌝ ∗
     ∀ e2 σ2 efs, ⌜head_step e1 σ1 κ e2 σ2 efs⌝ ={E1}[E2]▷=∗
-      ⌜efs = []⌝ ∗ state_interp σ2 κs n ∗ from_option Φ False (to_val e2))
+      ∃ δ2, ⌜valid_state_evolution AS σ1 δ1 κ σ2 δ2⌝ ∗
+      ⌜efs = []⌝ ∗ state_interp σ2 δ2 (κs ++ κ) n ∗
+      from_option Φ False (to_val e2))
   ⊢ WP e1 @ s; E1 {{ Φ }}.
 Proof.
   iIntros (?) "H". iApply wp_lift_atomic_head_step_fupd; [done|].
-  iIntros (σ1 κ κs Qs) "Hσ1". iMod ("H" $! σ1 with "Hσ1") as "[$ H]"; iModIntro.
+  iIntros (σ1 κ κs Qs st) "Hσ1".
+  iMod ("H" $! σ1 with "Hσ1") as "[$ H]"; iModIntro.
   iIntros (v2 σ2 efs Hstep).
   iMod ("H" $! v2 σ2 efs with "[# //]") as "H".
-  iIntros "!> !>". iMod "H" as "(-> & ? & ?) /=". by iFrame.
+  iIntros "!> !>". iMod "H" as (st') "(% & -> & ? & ?) /=".
+  iModIntro; iExists _; iSplit; first done.
+  iFrame.
 Qed.
 
 Lemma wp_lift_atomic_head_step_no_fork {s E Φ} e1 :
   to_val e1 = None →
-  (∀ σ1 κ κs n, state_interp σ1 (κ ++ κs) n ={E}=∗
+  (∀ σ1 δ1 κ κs n, state_interp σ1 δ1 κs n ={E}=∗
     ⌜head_reducible e1 σ1⌝ ∗
     ▷ ∀ e2 σ2 efs, ⌜head_step e1 σ1 κ e2 σ2 efs⌝ ={E}=∗
-      ⌜efs = []⌝ ∗ state_interp σ2 κs n ∗ from_option Φ False (to_val e2))
+      ∃ δ2, ⌜valid_state_evolution AS σ1 δ1 κ σ2 δ2⌝ ∗
+      ⌜efs = []⌝ ∗ state_interp σ2 δ2 (κs ++ κ) n ∗
+      from_option Φ False (to_val e2))
   ⊢ WP e1 @ s; E {{ Φ }}.
 Proof.
   iIntros (?) "H". iApply wp_lift_atomic_head_step; eauto.
-  iIntros (σ1 κ κs Qs) "Hσ1". iMod ("H" $! σ1 with "Hσ1") as "[$ H]"; iModIntro.
+  iIntros (σ1 κ κs Qs st) "Hσ1".
+  iMod ("H" $! σ1 with "Hσ1") as "[$ H]"; iModIntro.
   iNext; iIntros (v2 σ2 efs Hstep).
-  iMod ("H" $! v2 σ2 efs with "[//]") as "(-> & ? & ?) /=". by iFrame.
+  iMod ("H" $! v2 σ2 efs with "[//]") as (st') "(% & -> & ? & ?) /=".
+  iModIntro; iExists _; iSplit; first done.
+  iFrame.
 Qed.
 
 Lemma wp_lift_pure_det_head_step_no_fork {s E E' Φ} e1 e2 :
